equality subsessions

code/experimental/pkcs/Spec/Hacl.PKCS11.Specification.fst
@@ -630,32 +630,58 @@ assume val keyGeneration: mechanismID: _CK_MECHANISM ->
 )
 
 
+(* whether dependent variable should be also compares to be equal? *)
 
-val sessionEqual: #ks: seq keyEntity -> #ms: seq mechanismSpecification -> #ks1: seq keyEntity -> #ms1 : seq mechanismSpecification -> 
-	s: subSession ks ms -> s1 : subSession ks1 ms1 -> Tot Type0
+(* 
 
-let sessionEqual #ks #ms #ks1 #ms1 s s1 = 
-	match s with 
-	|Signature a b c d e -> 
-		begin match s1 with 
-			|Signature a1 b1 c1 d1 e1 -> a == a1 /\ b == b1 /\ c == c1 /\ d == d1 /\ e == e1
-			| _ -> False
-		end
-	|Verify a b c d e -> 	
-		begin 
-			match s1 with
-			| Verify a1 b1 c1 d1 e1 -> a == a1 /\ b == b1 /\ c == c1 /\ d == d1 /\ e == e1
-			| _ -> False
 
-		end	
+val sessionEqual: #ks: seq keyEntity -> #ms: seq _CK_MECHANISM -> #supM: seq _CKS_MECHANISM_INFO -> 
+  #ks1: seq keyEntity -> #ms1 : seq _CK_MECHANISM -> #supM1: seq _CKS_MECHANISM_INFO -> 
+  s: subSession ks ms supM -> s1 : subSession ks1 ms1 supM1 -> Tot Type0
 
+let sessionEqual #ks #ms #ks1 #ms1 #supM #supM1 s s1 = 
+  match s with 
+    |Signature a b c d e -> 
+      begin 
+	match s1 with 
+	  |Signature a1 b1 c1 d1 e1 -> a == a1 /\ b == b1 /\ c == c1 /\ d == d1 /\ e == e1
+	  | _ -> False
+      end
+    |Verify a b c d e -> 	
+      begin 
+	match s1 with
+	  | Verify a1 b1 c1 d1 e1 -> a == a1 /\ b == b1 /\ c == c1 /\ d == d1 /\ e == e1
+	  | _ -> False
+      end	
+*)
+
+(* compares two sessions -> The sessions are equal iff the dependencies are equal and the elements are equal *)
+val sessionEqual: #ks: seq keyEntity -> #ms: seq _CK_MECHANISM -> #supM: seq _CKS_MECHANISM_INFO -> 
+  #ks1: seq keyEntity -> #ms1 : seq _CK_MECHANISM -> #supM1: seq _CKS_MECHANISM_INFO -> 
+  s: subSession ks ms supM -> s1 : subSession ks1 ms1 supM1 -> Tot Type0
+
+let sessionEqual #ks #ms #supM  #ks1 #ms1 #supM1 s s1 = 
+  match s with 
+    |Signature a b c d e -> 
+      begin 
+	match s1 with 
+	  |Signature a1 b1 c1 d1 e1 -> ks == ks1 /\ ms == ms1 /\ supM == supM1 /\ a == a1 /\ b == b1 /\ c == c1 /\ d == d1 /\ e == e1
+	  | _ -> False
+      end
+    |Verify a b c d e -> 	
+      begin 
+	match s1 with
+	  | Verify a1 b1 c1 d1 e1 -> ks == ks1 /\ ms == ms1 /\ supM == supM1 /\ a == a1 /\ b == b1 /\ c == c1 /\ d == d1 /\ e == e1
+	  | _ -> False
+      end	
+
+(* This method recreated the session with the same parameters and dependecies *)
 val updateSession_: d: device -> 
-	s: subSession d.keys d.mechanisms ->
- 	ks: seq keyEntity{Seq.length ks >= Seq.length d.keys\/
- 		subSessionGetKeyHandler s < Seq.length ks} ->
-	ms: seq mechanismSpecification{ms == d.mechanisms} -> 
-	Tot (r: subSession ks ms
-		{Signature? s ==> Signature? r /\ Verify? s ==> Verify? r /\ sessionEqual s r})	
+  s: subSession d.keys d.mechanisms d.supportedMechanisms ->
+  ks: seq keyEntity {Seq.length ks >= Seq.length d.keys \/ subSessionGetKeyHandler s < Seq.length ks} ->
+  ms: seq mechanismSpecification{ms == d.mechanisms} -> 
+  Tot (r: subSession ks ms
+    {Signature? s ==> Signature? r /\ Verify? s ==> Verify? r /\ sessionEqual s r})	
 
 let updateSession_ d s ks ms = 
 	match s with 
